theories/caesium/heap.v
@@ -329,84 +329,13 @@ Proof.
   - solve_decision.
 Qed.
 
-(** ** Comparing pointers
-  [heap_loc_eq l1 l2] returns whether two pointers compare equal.
-  None means that the comparison is undefined. *)
-Definition heap_loc_eq (l1 l2 : loc) (st : heap_state) : option bool :=
-    (* null pointers are equal *)
-  if bool_decide (l1 = NULL_loc ∧ l2 = NULL_loc) then
-    Some true
-  (* function pointers are different from NULL pointers
-   TODO: Check that the address of the function pointer is not 0?*)
-  else if bool_decide ((l1 = NULL_loc ∧ l2.1 = ProvFnPtr) ∨ (l1.1 = ProvFnPtr ∧ l2 = NULL_loc)) then
-    Some false
-  (* Allocations are different from NULL pointers. But the comparison
-  is only defined if the location is in bounds of its allocation. *)
-  else if bool_decide (l1 = NULL_loc) then
-    guard (heap_state_loc_in_bounds l2 0 st);;
-    Some false
-  else if bool_decide (l2 = NULL_loc) then
-    guard (heap_state_loc_in_bounds l1 0 st);;
-    Some false
-  (* Two function pointers compare equal if their address is equal. *)
-  else if bool_decide (l1.1 = ProvFnPtr ∧ l2.1 = ProvFnPtr) then
-    Some (bool_decide (l1.2 = l2.2))
-  else
-  (* Two allocations can be compared if they are both alive and in
-  bounds (it is ok if they have different provenances). Comparison
-  compares the addresses. *)
-    guard (valid_ptr l1 st);;
-    guard (valid_ptr l2 st);;
-    Some (bool_decide (l1.2 = l2.2)).
-
-Lemma heap_loc_eq_symmetric l1 l2 st:
-  heap_loc_eq l1 l2 st = heap_loc_eq l2 l1 st.
-Proof.
-  rewrite /heap_loc_eq.
-  repeat case_bool_decide=> //; repeat case_guard => //; naive_solver.
-Qed.
-
-Lemma heap_loc_eq_NULL_NULL st:
-  heap_loc_eq NULL_loc NULL_loc st = Some true.
-Proof. rewrite /heap_loc_eq. case_bool_decide; naive_solver. Qed.
-
-Lemma heap_loc_eq_alloc_NULL l st:
-  heap_state_loc_in_bounds l 0 st →
-  heap_loc_eq l NULL_loc st = Some false.
-Proof.
-  move => Hlib. move: (Hlib) => /heap_state_loc_in_bounds_zero_or_has_alloc_id[[?[??]]|[??]];
-    rewrite /heap_loc_eq.
-  all: do 3 (case_bool_decide; [naive_solver|]).
-  all: case_bool_decide => //.
-  all: by rewrite option_guard_True.
-Qed.
-
-Lemma heap_loc_eq_fnptr_NULL l st:
-  l.1 = ProvFnPtr →
-  heap_loc_eq l NULL_loc st = Some false.
-Proof.
-  rewrite /heap_loc_eq => ?. do 3 (case_bool_decide; [naive_solver|]). naive_solver.
-Qed.
-
-Lemma heap_loc_eq_alloc_alloc l1 l2 st:
-  valid_ptr l1 st →
-  valid_ptr l2 st →
-  heap_loc_eq l1 l2 st = Some (bool_decide (l1.2 = l2.2)).
-Proof.
-  move => Hv1 Hv2. move: (Hv1) => /valid_ptr_is_alloc[[??]|?]; move: (Hv2) => /valid_ptr_is_alloc[[??]|?].
-  all: destruct l1, l2; simplify_eq/=.
-  all: rewrite /heap_loc_eq.
-  all: do 5 (case_bool_decide; [naive_solver|]).
-  all: by rewrite !option_guard_True.
-Qed.
-
 (** ** Converting a value to a boolean (for conditionals). *)
 
 Definition cast_to_bool (ot: op_type) (v: val) (st: heap_state) : option bool :=
   match ot with
   | BoolOp   => val_to_bool v
   | IntOp it => val_to_Z v it ≫= λ n, Some (bool_decide (n ≠ 0))
-  | PtrOp    => val_to_loc v ≫= λ l, heap_loc_eq l NULL_loc st ≫= λ b, Some (negb b)
+  (*| PtrOp    => val_to_loc v ≫= λ l, heap_loc_eq l NULL_loc st ≫= λ b, Some (negb b)*)
   | _        => None
   end.
 
